wip: gf128

code/experimental/gf128/Hacl.Gf128.NI.fst
@@ -11,9 +11,6 @@ open Hacl.Impl.Gf128.Fields
 open Hacl.Impl.Gf128.Generic
 
 module ST = FStar.HyperStack.ST
-
-module S = Spec.GF128
-module GF = Spec.GaloisField
 module Vec = Hacl.Spec.GF128.Vec
 
 #reset-options "--z3rlimit 50 --max_fuel 0 --max_ifuel 1"
@@ -25,70 +22,30 @@ let gcm_ctx_len = 5ul
 
 inline_for_extraction noextract
 let gcm_ctx_elem_zero = vec_zero U128 1
+inline_for_extraction noextract
 let gcm_ctx = lbuffer gcm_ctx_elem gcm_ctx_len
 
 
 [@CInline]
-val gcm_init:
-    ctx:gcm_ctx
-  -> key:lbuffer uint8 16ul ->
-  Stack unit
-  (requires fun h -> live h ctx /\ live h key /\ disjoint ctx key)
-  (ensures  fun h0 _ h1 -> modifies1 ctx h0 h1)
-
-let gcm_init ctx key = gcm_init #Vec.NI ctx key
+let gcm_init : gf128_init_st Vec.NI =
+  gf128_init #Vec.NI
 
 
 [@CInline]
-val gcm_update_blocks:
-    ctx:gcm_ctx
-  -> len:size_t
-  -> text:lbuffer uint8 len ->
-  Stack unit
-  (requires fun h -> live h ctx /\ live h text)
-  (ensures  fun h0 _ h1 -> modifies1 ctx h0 h1)
-
-let gcm_update_blocks ctx len text =
-  let acc = get_acc ctx in
-  let pre = get_precomp ctx in
-  gf128_update_vec #Vec.NI acc pre len text
+let gcm_update_blocks: gf128_update_st Vec.NI =
+  gf128_update #Vec.NI
 
 
 [@CInline]
-val gcm_update_padded:
-    ctx:gcm_ctx
-  -> len:size_t
-  -> text:lbuffer uint8 len ->
-  Stack unit
-  (requires fun h -> live h ctx /\ live h text)
-  (ensures  fun h0 _ h1 -> modifies1 ctx h0 h1)
-
-let gcm_update_padded ctx len text =
-  gcm_update_blocks ctx len text
+let gcm_update_padded: gf128_update_st Vec.NI =
+  gcm_update_blocks
 
 
 [@CInline]
-val gcm_emit:
-    tag:lbuffer uint8 16ul
-  -> ctx:gcm_ctx ->
-  Stack unit
-  (requires fun h -> live h ctx /\ live h tag)
-  (ensures  fun h0 _ h1 -> modifies1 tag h0 h1)
-
-let gcm_emit tag ctx =
-  let acc = get_acc ctx in
-  decode tag acc
+let gcm_emit: gf128_emit_st Vec.NI =
+  gf128_emit #Vec.NI
 
 
 [@CInline]
-val ghash:
-    tag:block
-  -> len:size_t
-  -> text:lbuffer uint8 len
-  -> key:block ->
-  Stack unit
-  (requires fun h -> live h tag /\ live h text /\ live h key)
-  (ensures  fun h0 _ h1 -> modifies1 tag h0 h1)
-
-let ghash tag len text key =
-  ghash #Vec.NI tag len text key
+let ghash: ghash_st Vec.NI =
+  ghash #Vec.NI
